---
title: Inverse of a Transposed Matrix
author: jModeler
date: '2025-05-12'
slug: []
categories:
  - math
tags: []
authors: []
description: ''
externalLink: ''
series: []
math: true
nocite: '@*'
---

In this post I attempt to prove a very simple identity, that will be used in a later post.

I want to prove that for a square, non-singular matrix $A$, we have (in the steps below, $I$ is the identity matrix:

\begin{align}
(A^T)^{-1} = (A^{-1})^{T}
\end{align}

Let $(A^T)^{-1} = B$, we have
\begin{align}
(A^T)^{-1} & = B \\
\implies (A^T)^{-1} A^T & = B A^T \\
\implies I & = B A^T  (\#eq:multinv)  \\
\implies I^T & = (BA^T)^T \\
\implies I & = AB^T (\#eq:transmat) \\
\implies A^{-1}I & = A^{-1}AB^T \\
\implies A^{-1} & = B^T \\
\implies (A^{-1})^T & = (B^T)^T \\
\implies (A^{-1})^T & = B \\
\implies (A^{-1})^T & = B = (A^T)^{-1}
\end{align}

This completes the proof. I use the following identities in the labeled equations above:

- Equation \@ref(eq:multinv) A square, non singular matrix multiplied by its inverse is the identity matrix $(A^T)^{-1} A^T  = I$
- Equation \@ref(eq:transmat) comes from the [transpose of a matrix product](https://en.wikipedia.org/wiki/Transpose#Products) identity. $(BA^T)^T = AB^T$